solvers/1.lean
@@ -1,12 +1,18 @@
+import ProjectEulerStatements.P1
+
 def sumOfMultiples (m n : Nat) : Nat :=
   let k := n / m
   (m * k * (k + 1)) / 2
 
-def sumOfMultiplesOfEither3Or5 (n : Nat) : Nat :=
+def p1sol (n : Nat) : Nat :=
   let n' := n - 1
   sumOfMultiples 3 n' + sumOfMultiples 5 n' - sumOfMultiples 15 n'
 
-example : sumOfMultiplesOfEither3Or5 10 = 23 := rfl
+example : p1sol 10 = 23 := rfl
+
+theorem p1_10 : p1sol 10 = 23 := by native_decide
+theorem p1 : p1sol 1000 = 233168 := by native_decide
+theorem p1_equiv (n : ℕ) : p1def n = p1sol n := sorry
 
 def main : IO Unit := do
-  IO.println (sumOfMultiplesOfEither3Or5 1000)
+  IO.println (p1sol 1000)
